

Topic to discuss

→ Proof / Derive Newton Forward Interpolation formula.

YouTube @StartPracticing

Proof Newton Forward Interpolation Formula

Let $y = f(x)$ be a function.
and x_0, x_1, x_2, \dots are the
equidistant data point.

Let h is the step length or
constant difference between
two successive value of x .

$$\Rightarrow h = x_1 - x_0$$

we know, $y = f(x)$

$$y_0 = f(x_0)$$

$$y_1 = f(x_1) = f(x_0 + h)$$

$$y_2 = f(x_2) = f(x_0 + 2h)$$

\vdots

and so on.

x	$y = f(x) = y(x)$
x_0	y_0
$x_1 = x_0 + h$	y_1
$x_2 = x_0 + 2h$	y_2
$x_3 = x_0 + 3h$	y_3
\vdots	\vdots
$x_n = x_0 + nh$	y_n

Suppose x is interpolation point and we want to find function value of x which is $f(x)$. and close to top of the given data point.

We know, $y = f(x) = y(x)$

and, $x = x_0 + uh$

$$\Rightarrow u = \frac{x - x_0}{h}$$

Step-1:

We know, Forward Shift Operator E such that

$$Ef(x) = f(x+h)$$

$$E^u f(x) = f(x+uh) \quad [\text{Replace } x \rightarrow x_0]$$

$$\Rightarrow E^u f(x_0) = f(x_0 + uh)$$

$$\Rightarrow E^u y_0 = f(x)$$

$$\Rightarrow f(x) = E^u y_0$$

$$f(x) = E^u y_0 \quad [E = 1 + \Delta \quad ; \Delta \text{ is forward difference operator}]$$

$$f(x) = (1 + \Delta)^u y_0 \quad \text{--- (1)}$$

Step-2

We know Binomial Expansion Theorem such that,

$$(1+x)^n = 1 + nx + \frac{n(n-1)}{2!} x^2 + \frac{n(n-1)(n-2)}{3!} x^3 + \dots$$

Applying this in equation --- (1)

$$f(x) = (1 + \Delta)^u y_0$$

$$f(x) = \left[1 + u\Delta + \frac{u(u-1)}{2!} \Delta^2 + \frac{u(u-1)(u-2)}{3!} \Delta^3 + \dots \right] y_0$$

$$f(x) = y_0 + u\Delta y_0 + \frac{u(u-1)}{2!} \Delta^2 y_0 + \frac{u(u-1)(u-2)}{3!} \Delta^3 y_0 + \dots$$

(Proved)

Connect with me



[Start Practicing](#)



[i._am._arfin](#)



[Arfin Parween](#)



[Arfin Parween \(Subscribe here too\)](#)



[Arfin Parween](#)



[Arfin Parween](#)